prove lookup

Scratch.thy
@@ -2,22 +2,9 @@ theory Scratch
   imports Main "Separation_Logic_Imperative_HOL.Sep_Main" "Deriving.Derive" "HOL-Library.Code_Target_Nat"
 begin
 
-(**
 
-   'a cell = Array 'a array | Upd nat 'a ('a cell ref)
-
-   'a la = 'a cell ref ref
-
-*)
-find_consts "_ set" name: fold
-find_theorems "Finite_Set.fold _ _ (insert _ _)"
-find_theorems "comp_fun_commute_on" "Finite_Set.fold"
-
-
-interpretation mf: comp_fun_commute_on UNIV "((*)::_::comm_monoid_mult \<Rightarrow> _)"
-  apply(unfold_locales)
-  by(auto simp: algebra_simps)
-
+abbreviation member where
+  "member xs x \<equiv> x \<in> set xs"
 
 definition fold_assn :: "assn list \<Rightarrow> assn" where
   "fold_assn assns = foldr (*) assns emp"
@@ -34,12 +21,11 @@ lemma fold_assn_app [simp]: "fold_assn (xs@ys) = fold_assn xs * fold_assn ys"
   apply(induction xs)
   by(auto simp: algebra_simps)
 
-lemma fold_assn_remove1: "List.member xs x \<Longrightarrow> fold_assn xs = x * fold_assn (remove1 x xs)"
-  unfolding member_def
+lemma fold_assn_remove1: "member xs x \<Longrightarrow> fold_assn xs = x * fold_assn (remove1 x xs)"
   apply(induction xs)
   by(auto simp: algebra_simps)
 
-lemma fold_assn_false [simp]: "List.member xs false \<Longrightarrow> fold_assn xs = false"
+lemma fold_assn_false [simp]: "member xs false \<Longrightarrow> fold_assn xs = false"
   using fold_assn_remove1
   by auto
 
@@ -51,38 +37,10 @@ lemma fold_assn_emp_removeAll: "fold_assn xs = fold_assn (removeAll emp xs)"
   apply(induction xs)
   by auto  
 
-(*
-definition fold_assn :: "assn set \<Rightarrow> assn" where
-  "fold_assn assns = Finite_Set.fold (*) emp assns * \<up>(finite assns)"
-
-lemma fold_assn_emp [simp]: "fold_assn {} = emp"
-  unfolding fold_assn_def
-  by simp
-
-lemma fold_assn_false: "false \<in> S \<Longrightarrow> fold_assn S = false"
-  unfolding fold_assn_def
-  apply(cases "finite S")
-  by(auto simp: mf.fold_rec)
-
-lemma fold_assn_emp': "emp \<in> S \<Longrightarrow> fold_assn S = fold_assn (S - {emp})"
-  unfolding fold_assn_def
-  apply(cases "finite S")
-  by(auto simp: mf.fold_rec)
-
-thm  mf.fold_insert_remove
-*)
-lemma fold_assn_cons [simp]: "fold_assn (insert x xs) = x * fold_assn (xs - {x})"
-  unfolding fold_assn_def
-  apply(cases "finite xs")
-  by(simp_all add: mf.fold_insert_remove)
-
-lemma fold_assn_in: "x \<in> xs \<Longrightarrow> fold_assn xs = x * fold_assn (xs - {x})"
-  by (metis fold_assn_cons insert_absorb)
-*)
-
-(*lemma fold_assn_app: "fold_assn (xs \<union> ys) = fold_assn xs * fold_assn ys"
+lemma fold_assn_map: "member xs x \<Longrightarrow> fold_assn (remove1 (f x) (map f xs)) = fold_assn (map f (remove1 x xs))"
   apply(induction xs)
-  by(auto simp: algebra_simps)*)
+  apply auto
+  by (metis fold_assn_remove1 image_eqI list.set_map)
 
 datatype 'a::"countable" cell = Array "'a array" | Upd nat "'a" "'a cell ref"
 
@@ -103,147 +61,34 @@ fun cell_assn where
 | "cell_assn (Upd' i' val' p') (Upd i val p) = \<up>(i = i' \<and> val = val' \<and> p = p')"
 | "cell_assn _ _ = false"
 
-(* remove1 *)
-
 
 definition master_assn :: "('a cell ref * 'a::heap cell') list \<Rightarrow> assn" where
   "master_assn C = fold_assn (map (\<lambda>(p, c'). \<exists>\<^sub>A c. p \<mapsto>\<^sub>r c * cell_assn c' c) C)"
-
-
-(*lemma test: "(p, c) \<in> Map.graph C \<Longrightarrow> Map.graph C - { (p, c) } =  Map.graph (C (p := None))"
-  by (metis (mono_tags, lifting) Diff_insert_absorb fun_upd_same fun_upd_triv graph_map_upd in_graphD option.simps(3))
-
-lemma test_2: "\<lbrakk>
-    inj_on f (Map.graph C); (k, v) \<in> Map.graph C; 
-    (k', v') \<in> Map.graph (C(k := None)); 
-    f (k', v') = f (k, v)
-\<rbrakk> \<Longrightarrow> False"
-  by (metis Diff_iff inj_on_contraD singletonI test)
-
-lemma test_3: "\<lbrakk>inj_on f (Map.graph C); (k, v) \<in> Map.graph C\<rbrakk>
-   \<Longrightarrow> f ` Map.graph C - { f (k, v) } = f ` Map.graph (C(k := None))"
-  apply(auto)
-  apply (metis image_eqI insert_Diff insert_iff test)
-  apply (metis DiffE rev_image_eqI test)
-  by (meson test_2)
-
-lemma test_5_1: "(cell_assn x z = cell_assn y z \<Longrightarrow> x = y) \<Longrightarrow> (cell_assn x = cell_assn y \<Longrightarrow> x = y)"
-  by auto
-
-lemma test21: "\<lbrakk>h \<Turnstile> a \<mapsto>\<^sub>r c * cell_assn b c; h \<Turnstile> aa \<mapsto>\<^sub>r ca * cell_assn ba ca\<rbrakk> \<Longrightarrow> a = aa"
-  unfolding sngr_assn_def
-  apply(induction b c rule: cell_assn.induct)
-     apply auto
-   apply(induction ba ca rule: cell_assn.induct)
-      apply auto
-    apply(induction a; induction aa)
-    apply auto
-  unfolding snga_assn_def
-    apply(induction h)
-  apply auto   
-  sorry
-
-lemma test20: "(\<exists>c. h \<Turnstile> a \<mapsto>\<^sub>r c * cell_assn b c) = (\<exists>c. h \<Turnstile> aa \<mapsto>\<^sub>r c * cell_assn ba c)
-   \<Longrightarrow>  a = aa"
-  apply auto
-  sorry
-
-lemma test19: "(\<lambda>h. \<exists>c. h \<Turnstile> a \<mapsto>\<^sub>r c * cell_assn b c) = (\<lambda>h. \<exists>c. h \<Turnstile> aa \<mapsto>\<^sub>r c * cell_assn ba c)
-   \<Longrightarrow> (\<exists>c. h \<Turnstile> a \<mapsto>\<^sub>r c * cell_assn b c) = ( \<exists>c. h \<Turnstile> aa \<mapsto>\<^sub>r c * cell_assn ba c)"
-  by meson
-
-lemma test17: "
-   Abs_assn (\<lambda>h. \<exists>c. h \<Turnstile> a \<mapsto>\<^sub>r c * cell_assn b c) = Abs_assn (\<lambda>h. \<exists>c. h \<Turnstile> aa \<mapsto>\<^sub>r c * cell_assn ba c) \<Longrightarrow> (\<lambda>h. \<exists>c. h \<Turnstile> a \<mapsto>\<^sub>r c * cell_assn b c) = (\<lambda>h. \<exists>c. h \<Turnstile> aa \<mapsto>\<^sub>r c * cell_assn ba c)"
-  by (smt (verit, ccfv_threshold) Abs_assn_inverse mem_Collect_eq mod_relH models_in_range proper_def)
-
-lemma test18: "(\<lambda>h. \<exists>c. h \<Turnstile> a \<mapsto>\<^sub>r c * cell_assn b c) = (\<lambda>h. \<exists>c. h \<Turnstile> aa \<mapsto>\<^sub>r c * cell_assn ba c) \<Longrightarrow> a = aa" 
-  sorry
-
-lemma test15:  "(\<exists>\<^sub>Ac. a \<mapsto>\<^sub>r c * cell_assn b c) = (\<exists>\<^sub>Ac. aa \<mapsto>\<^sub>r c * cell_assn ba c) \<Longrightarrow> a = aa"
-  using test18[of a b aa ba]
-  unfolding ex_assn_def
-  using test17 by blast
-
-lemma test14: "inj (\<lambda>x. case x of (p, c') \<Rightarrow> \<exists>\<^sub>Ac. p \<mapsto>\<^sub>r c * cell_assn c' c)"
-  apply(auto simp: inj_def test15 exI)
-  sorry
-
-lemma test_7: "(p, c') \<in> Map.graph C \<Longrightarrow>
-    Finite_Set.fold g acc (f ` Map.graph C)  =
-    g (f (p, c')) (Finite_Set.fold g acc (f ` Map.graph (C(p := None))))"
-  apply auto
- sorry
-
-lemma test_6: "(p, c') \<in> Map.graph C \<Longrightarrow>
-    fold_assn (f ` Map.graph C) = (f (p, c') * fold_assn (f ` Map.graph (C(p := None))))" 
-  unfolding fold_assn_def
-  apply auto
-  sorry
-
-lemma "a \<mapsto>\<^sub>a xs = false \<Longrightarrow> False"
-  unfolding snga_assn_def
-  apply(induction a)
-  sorry
-
-lemma test_5_2: "cell_assn x z = cell_assn y z \<Longrightarrow> x = y"
-  apply(induction x z rule: cell_assn.induct; induction y z rule: cell_assn.induct)
-  apply auto
-  sorry
-
-lemma test_5: "inj cell_assn" 
-  unfolding inj_def
-  apply auto
-  subgoal for x y
-    apply(induction x; induction y)
-       apply auto
-    sorry
-  sorry
-  
-
-lemma test_4_3: "h \<Turnstile> p \<mapsto>\<^sub>r a * F \<and>\<^sub>A p \<mapsto>\<^sub>r a' * F' \<longrightarrow> a = a'"
-  using sngr_prec
-  unfolding precise_def
-  by blast
-
-lemma test_4_2: "precise (\<lambda>c' p. \<exists>\<^sub>Ac. p \<mapsto>\<^sub>r c)"
-  unfolding precise_def
-  apply auto
-  subgoal for a b p F Fa x xa aa xb
-    using test_4_3[of p xa F x Fa "(a, b)"]
-    apply auto
-    sorry
-  sorry
-  
-
-lemma test_4_1: "\<lbrakk>(\<exists>\<^sub>Ac. a \<mapsto>\<^sub>r c * cell_assn b c) = (\<exists>\<^sub>Ac. aa \<mapsto>\<^sub>r c * cell_assn ba c)\<rbrakk> \<Longrightarrow> a = aa"
-  using sngr_prec
-  unfolding precise_def
-  apply sep_auto
-  sorry
-
-lemma test_4: "inj_on (\<lambda>x. case x of (p, c') \<Rightarrow> \<exists>\<^sub>Ac. p \<mapsto>\<^sub>r c * cell_assn c' c) (Map.graph C)"
-  unfolding inj_on_def
-  apply auto
-  using test_4_1
-  sorry
-*)
 
 
 lemma open_master_assn': "master_assn ((p,c')#xs) = (\<exists>\<^sub>A c. p \<mapsto>\<^sub>r c * cell_assn c' c) * master_assn xs"
   unfolding master_assn_def
   by auto
 
+lemma open_master_assn: 
+  assumes "member xs (p, c')"
+  shows "master_assn xs = (\<exists>\<^sub>A c. p \<mapsto>\<^sub>r c * cell_assn c' c) * master_assn (remove1 (p, c') xs)"
+proof-
+  from assms have 
+    "member (map (\<lambda>(p, c'). \<exists>\<^sub>Ac. p \<mapsto>\<^sub>r c * cell_assn c' c) xs) (\<exists>\<^sub>A c. p \<mapsto>\<^sub>r c * cell_assn c' c)"
+    by auto
 
-lemma open_master_assn: "List.member xs  (p, c') \<Longrightarrow> master_assn xs = (\<exists>\<^sub>A c. p \<mapsto>\<^sub>r c * cell_assn c' c) * master_assn (remove1 (p, c') xs)"
-  unfolding master_assn_def member_def
-  apply auto
-  sledgehammer
-  sorry
-
+  with assms show ?thesis
+    unfolding master_assn_def
+    using 
+        fold_assn_remove1
+        fold_assn_map[of "(p, c')" xs "(\<lambda>(p, c'). \<exists>\<^sub>Ac. p \<mapsto>\<^sub>r c * cell_assn c' c)"]
+    by auto
+qed 
 
 fun la_rel' where
-  "la_rel' C 0 xs a \<longleftrightarrow> List.member C (a, Array' xs)"
-| "la_rel' C (Suc n) xs a \<longleftrightarrow> (\<exists>i x a' xs'. List.member C (a, Upd' i x a') \<and> la_rel' C n xs' a' \<and> xs = xs'[i:=x])"
+  "la_rel' C 0 xs a \<longleftrightarrow> member C (a, Array' xs)"
+| "la_rel' C (Suc n) xs a \<longleftrightarrow> (\<exists>i x a' xs'. member C (a, Upd' i x a') \<and> la_rel' C n xs' a' \<and> xs = xs'[i:=x])"
   
 definition la_rel where
   "la_rel C xs a \<equiv> \<exists>n. la_rel' C n xs a"
@@ -274,7 +119,6 @@ partial_function (heap) lookup :: "('a::heap) la  \<Rightarrow> nat \<Rightarrow
   }"
 declare lookup.simps[code]
 
-
 lemma [simp]:"cell_assn (Array' xs) c = (\<exists>\<^sub>Aa. \<up>(c = Array a) * a \<mapsto>\<^sub>a xs)"
   apply(cases c)
    apply(auto)
@@ -285,38 +129,75 @@ lemma [simp]:"cell_assn (Upd' i x p) c = \<up>(c = Upd i x p)"
   apply(cases c)
   by auto
 
+lemma close_master_assn_array: "member t (a, Array' xs) 
+  \<Longrightarrow> a' \<mapsto>\<^sub>a xs * a \<mapsto>\<^sub>r cell.Array a' * master_assn (remove1 (a, Array' xs) t) \<Longrightarrow>\<^sub>A master_assn t"
+  using open_master_assn[of a "Array' xs" t]
+  by sep_auto
 
+lemma close_master_assn_upd: "member t (a, Upd' i x a')
+     \<Longrightarrow> a \<mapsto>\<^sub>r Upd i x a' * master_assn (remove1 (a, Upd' i x a') t) \<Longrightarrow>\<^sub>A master_assn t"
+  using open_master_assn[of a "Upd' i x a'" t]
+  by sep_auto
 
-lemma close_master_assn_upd: "a \<mapsto>\<^sub>r Upd i x a' * master_assn (remove1 (a, Upd' i x a') t) \<Longrightarrow>\<^sub>A master_assn t"
-  unfolding master_assn_def
-  using open_master_assn
-  sorry
+lemma close_master_assn_upd': "member t (a, Upd' i x a')
+     \<Longrightarrow> a \<mapsto>\<^sub>r Upd i x a' * master_assn (remove1 (a, Upd' i x a') t) = master_assn t"
+  using open_master_assn[of a "Upd' i x a'" t]
+  by(auto simp: ent_iffI entails_def)
+
+(* How to inline these? *)
+lemma helper1:
+  assumes 
+    "i < length xs'"
+    "member t (a, Upd' i x a')"
+    "la_rel' t n xs' a'"
+    "xs = xs'[i := x]"
+  shows
+    "a \<mapsto>\<^sub>r Upd i x a' * master_assn (remove1 (a, Upd' i x a') t) \<Longrightarrow>\<^sub>A master_assn t * true"
+proof-  
+  from assms show ?thesis 
+    using close_master_assn_upd[of a i x a' t]
+    apply sep_auto
+    using ent_true_drop(2) by blast
+qed
+
+lemma helper2: 
+  assumes
+     "i < length xs'" 
+     "member t (a, Upd' ia x a')" 
+     "la_rel' t n xs' a'" 
+     "xs = xs'[ia := x]"
+     "i \<noteq> ia"
+   shows "
+      <a \<mapsto>\<^sub>r Upd ia x a' * master_assn (remove1 (a, Upd' ia x a') t)> lookup a' i <\<lambda>r. master_assn t * true * \<up> (r = xs' ! i)>
+       = <master_assn t> lookup a' i <\<lambda>x. master_assn t * true * \<up> (x = xs' ! i)>"
+  using close_master_assn_upd'[of a ia x a' t] assms
+  by auto
 
 lemma lookup: "<master_assn t * \<up>(la_rel' t n xs a \<and> i < length xs)> lookup a i <\<lambda>r. master_assn t * \<up>(r = xs!i)>\<^sub>t"
 proof(induction n arbitrary: xs a)
   case 0
+  then have "\<And>a'. \<lbrakk>member t (a, Array' xs); i < length xs\<rbrakk>
+         \<Longrightarrow> a' \<mapsto>\<^sub>a xs * a \<mapsto>\<^sub>r cell.Array a' * master_assn (remove1 (a, Array' xs) t) \<Longrightarrow>\<^sub>A master_assn t"
+    using close_master_assn_array
+    by sep_auto
+
   then show ?case
     apply(sep_auto)
     apply(subst lookup.simps)
     apply(subst open_master_assn, assumption)
-    apply(sep_auto simp: List.member_def)
-    (*apply (rule ent_frame_fwd[OF close_master_assn_upd], frame_inference)*)
-     sorry
+    apply(sep_auto)
+    using ent_true_drop(2) by blast
 next
   case (Suc n)
+
   show ?case
     apply(sep_auto)
     apply(subst lookup.simps)
     apply(subst open_master_assn, assumption)
-    apply(sep_auto)
-    apply (rule ent_frame_fwd[OF close_master_assn_upd], frame_inference)
-    apply sep_auto
-    apply(rule cons_pre_rule[OF close_master_assn_upd])
+    apply(sep_auto simp: helper1 helper2)
     apply (rule cons_post_rule)
     apply (rule fi_rule[OF Suc.IH])
-    apply sep_auto
-    apply sep_auto
-    done
+    by sep_auto+
 qed
 
 partial_function (heap) update :: "('a::heap) la \<Rightarrow> nat \<Rightarrow> 'a::heap \<Rightarrow> 'a la Heap" where
@@ -335,15 +216,15 @@ partial_function (heap) update :: "('a::heap) la \<Rightarrow> nat \<Rightarrow>
   }"
 declare update.simps[code]
 
-definition array_to_la' where
-  "array_to_la' n x = do {
+definition create_la where
+  "create_la n x = do {
     a \<leftarrow> Array.new n x;
     Array.upd 0 (42::nat) a;
     array_to_la a
   }"
 
 definition test where "test = do {
-  r \<leftarrow> array_to_la' 3 (5::nat);
+  r \<leftarrow> create_la 3 (5::nat);
   y \<leftarrow> update r 1 (6::nat);
   x \<leftarrow> lookup y 2;
   return x
